Clean/Gadgets/Addition32/Addition32Full.lean
@@ -91,7 +91,7 @@ theorem soundness : Soundness (F p) elaborated assumptions spec := by
 
   -- simplify circuit
   simp only [circuit_norm, subcircuit_norm, add32_full, add8_full_carry, Boolean.circuit, ByteLookup] at h
-  simp only [h_inputs, ByteTable.equiv] at h
+  simp only [h_inputs, ByteTable.equiv, and_assoc] at h
   repeat rw [add_neg_eq_zero] at h
   set z0 := env.get i0
   set c0 := env.get (i0 + 1)
@@ -140,7 +140,7 @@ theorem completeness : Completeness (F p) elaborated assumptions := by
 
   -- simplify circuit
   dsimp only [circuit_norm, subcircuit_norm, add32_full, add8_full_carry, Boolean.circuit] at henv ⊢
-  simp only [h_inputs, circuit_norm, subcircuit_norm] at henv ⊢
+  simp only [h_inputs, circuit_norm, subcircuit_norm, and_assoc] at henv ⊢
 
   -- characterize local witnesses
   obtain ⟨ hz0, hc0, hz1, hc1, hz2, hc2, hz3, hc3 ⟩ := henv
